\documentclass[12pt]{article}
\usepackage[margin = 1in]{geometry}
\usepackage{amsmath}
\usepackage{amssymb}
\usepackage{amsthm}
\usepackage{graphicx}
\usepackage{subfig}
\usepackage{enumitem}

\begin{document}
	
	\begin{center}
		\textbf{Quiz 9} \\
		\textbf{Differential Equations} \\
		\textbf{Math 337} \\
		\textbf{Stephen Giang} \\
	\end{center}

\noindent \textbf{Problem 1: }Suppose that $f(t)$ has a \textit{Laplace Transform} $F(s) = \mathcal{L}[f(t)]$, where 
	$$
	F(s) = \frac{12}{s^3} + \frac{16}{s^2 + 9} + \frac{20s}{(s+1)^2 + 4} 
	$$
Find $f(t)$
\\ \\
To find $f(t)$, we need to take the Laplace inverse of each term:
	$$
	f(t) = 6t^2 + \frac{16\sin(3t)}{3} + 20e^{-t}\cos(2t)
	$$
	
\newpage

\noindent \textbf{Problem 2: }Suppose that $f(t)$ has a \textit{Laplace Transform} $F(s) = \mathcal{L}[f(t)]$, where
	$$
	F(s) = \frac{3s^2 + 8s + 80}{s^2(s^2 - 6s + 40)}
	$$
Find $f(t)$
\\ \\
Notice the following:
	\begin{align*}
		F(s) = \frac{3}{(s-3)^2 + 31} + \frac{8}{s(s^2 - 6s + 40)} + \frac{80}{s^2(s^2 - 6s + 40)}
	\end{align*}	
Notice the partial fractions decomposition:
	\begin{align*}
		\frac{8}{s(s^2 - 6s + 40)} &= \frac{A}{s} + \frac{Bs + C}{s^2 - 6s + 40} \\
		8 &= (A+B)s^2 + (-6A + C)s + 40A 
	\end{align*}
So we can see that $A = \frac{1}{5}, B  = \frac{-1}{5}, C = \frac{6}{5}$
	\begin{align*}
	\frac{8}{s(s^2 - 6s + 40)} &= \frac{1}{5s} + \frac{-s + 6}{5(s^2 - 6s + 40)} \\
	&= \frac{1}{5s} - \frac{s-3}{5((s-3)^2 + 31)} + \frac{9}{5((s-3)^2 + 31)}
	\end{align*}
Notice another partial fractions decomposition:
	\begin{align*}
		\frac{80}{s^2(s^2 - 6s + 40)} &= \frac{A}{s} + \frac{B}{s^2} + \frac{Cs + D}{s^2 - 6s + 40} \\
		80 &= As^3 - 6As^2 + 40As + Bs^2 - 6Bs + 40B + Cs^3 + Ds^2 \\
		&= (A+C)s^3 + (-6A + B + D)s^2 + (40A - 6B)s + 40B
	\end{align*}
So we can see that $B = 2, A = \frac{3}{10}, D= \frac{-2}{10}, C = \frac{-3}{10}$
	\begin{align*}
		\frac{80}{s^2(s^2 - 6s + 40)} = \frac{3}{10s} + \frac{2}{s^2} - \frac{3(s-3)}{10((s-3)^2 + 31)} - \frac{11}{10((s-3)^2 + 31)}
	\end{align*}
\\ \\
After resubstitution, we get:
	\begin{align*}
		F(s) &= \frac{3}{(s-3)^2 + 31} + \frac{1}{5s} - \frac{s-3}{5((s-3)^2 + 31)} + \frac{9}{5((s-3)^2 + 31)} \\
		&+ \frac{3}{10s} + \frac{2}{s^2} -  \frac{3(s-3)}{10((s-3)^2 + 31)} - \frac{11}{10((s-3)^2 + 31)}
	\end{align*} 
After taking the Laplace inverse of each term, we get:
	\begin{align*}
		f(t) &= \frac{3\sin(\sqrt{31}t)e^{3t}}{\sqrt{31}} + \frac{1}{5} - \frac{\cos(\sqrt{31}t)e^{3t}}{5} + \frac{9\sin(\sqrt{31}t)e^{3t}}{5\sqrt{31}} + \frac{3}{10} + 2t \\
		&= \frac{3\cos(\sqrt{31}t)e^{3t}}{10} + \frac{11\sin(\sqrt{31}t)e^{3t}}{10\sqrt{31}}
	\end{align*}
	
\newpage 

\noindent \textbf{Problem 3: }Solve the following initial value problem with \textit{Laplace transforms}:
	$$
	y'' - 4y' + 8y = 20\cos(2t), \qquad y(0) = 5, \qquad y'(0) = 6.
	$$
So we need to take the Laplace transform of each side:
	\begin{align*}
		\mathcal{L}[y'' - 4y' + 8y] &= s^2Y(s) -sy(0) - y'(0) - 4sY(s) + 4y(0) + 8Y(s) \\
		&= (s^2 - 4s + 8)Y(s) - (5s - 14) \\
		\mathcal{L}[20\cos(2t)] &= \frac{20s}{s^2 + 4}
	\end{align*}
So we get the following equality:
	\begin{align*}
		Y(s) = \frac{20s}{(s^2 + 4)(s^2 - 4s + 8)} + \frac{5s - 14}{s^2 - 4s + 8}
	\end{align*}
Notice the partial fractions decomposition:
	\begin{align*}
		\frac{20s}{(s^2 + 4)(s^2 - 4s + 8)} &= \frac{As + B}{s^2 + 4} + \frac{Cs + D}{s^2 - 4s + 8} \\
		20s &= (A+C)s^3 + (-4A + B + D)s^2 + (8A - 4B + 4C)s + (8B + 4D)
	\end{align*}	
We can solve the following using system of equations:
	\begin{align*}
		A + C &= 0 \\
		-4A + B + D &= 0 \\
		8A - 4B + 4C &= 20 \\
		8B + 4D &= 0
	\end{align*}
Using matrix reduction, we get $A = 1, B = -4, C = -1, D = 8$.
	$$
	\frac{20s}{(s^2 + 4)(s^2 - 4s + 8)} = \frac{s - 4}{s^2 + 4} - \frac{s - 8}{s^2 - 4s + 8}
	$$
So we get the following after some algebra:
	\begin{align*}
		Y(s) &= \frac{s - 4}{s^2 + 4} - \frac{s - 8}{s^2 - 4s + 8} + \frac{5s - 14}{s^2 - 4s + 8} \\
		&= \frac{s}{s^2 + 4} - \frac{4}{s^2 + 4} - \frac{s - 2}{(s-2)^2 + 4} + \frac{6}{(s-2)^2 + 4} + \frac{5(s-2)}{(s-2)^2 + 4} - \frac{4}{(s-2)^2 + 4} \\
		&= \frac{s}{s^2 + 4} - \frac{4}{s^2 + 4} + \frac{4(s - 2)}{(s-2)^2 + 4} + \frac{2}{(s-2)^2 + 4}
	\end{align*}
Now we take Laplace inverse of each term and get:
	$$
	y(t) = \cos(2t) - 2\sin(2t) +  4\cos(2t)e^{2t} + \sin(2t)e^{2t} 
	$$
	
	
	
	
	
	
	
	
	
	
	
	
	
	
	
	
	
	
	
	
\end{document}
