\documentclass[12pt]{article}
\usepackage[margin = 1in]{geometry}
\usepackage{amsmath}
\usepackage{amssymb}
\usepackage{amsthm}
\usepackage{graphicx}
\usepackage{subfig}
\usepackage{enumitem}

\begin{document}
	
	\begin{center}
		\textbf{SecondDE} \\
		\textbf{Differential Equations} \\
		\textbf{Math 337} \\
		\textbf{Stephen Giang} \\
	\end{center}

\noindent \textbf{Problem 9: }Find the Solution for
	\begin{align*}
		y'' + 7y' + 10y = 36e^t && y(0) = 4, y'(0) = 1 
	\end{align*}
To find the eigenvalues, we can write the equation like below and solve for $\lambda$.
	\begin{align*}
		\lambda^2 + 7\lambda + 10 &= (\lambda + 5)(\lambda + 2) = 0 	\\
		\lambda &= -5, -2 				
	\end{align*}
Now we can write the homogeneous solution as: 
	$$
	y_h = c_1e^{-5t} + c_2e^{-2t}
	$$
To solve for the particular solution, we can write $y_p$ as below
	\begin{align*}
		y_p' = Ae^t &&&
		y_p' = Ae^t &&&
		y_p'' = Ae^t 
	\end{align*}
By plugging in the particular solution:
	\begin{align*}
		y_p'' + 7y_p' + 10y_p &= Ae^t + 7Ae^t + 10Ae^t \\
		18Ae^t &= 36e^t \\
		A &= 2 
	\end{align*}
So thus the particular solution is: 
	$$
	y_p = 2e^t
	$$
We can now have the complete solution, $y(t)$ to this differential equation:
	$$
	y(t)= c_1e^{-5t} + c_2e^{-2t} + 2e^t
	$$
We now use $y'(t)$ and the initial conditions to solve for $c_1$ and $c_2$
	$$
	y'(t) = -5c_1e^{-5t} + -2c_2e^{-2t} + 2e^t
	$$
	\begin{align*}
		y(0)&= c_1 + c_2 + 2 = 4 \\
		y'(0) &= -5c_1 + -2c_2 + 2 = 1 
	\end{align*}
	\begin{align*}
		\text{rref}\begin{pmatrix}
			1 & 1 & 2 \\
			-5 & -2 & -1
		\end{pmatrix} &= 
		\begin{pmatrix}
			1 & 0 & -1 \\
			0 & 1 & 3
		\end{pmatrix}
	\end{align*}
Thus the solution is: 
	$$
	y(t) = -e^{-5t} + 3e^{-2t} + 2e^t
	$$
	
\newpage 

\noindent \textbf{Problem 14: }Write a complete solution with details on how you found the general solution
	$$
	y'' + 16y = -16\sin(4t)
	$$
To solve for the particular solution, we can write $y_p$ as below
	\begin{align*}
		y_p &= At\cos \left( 4\,t \right) +Bt\sin \left( 4\,t \right) \\
		y_p'&= A\cos \left( 4\,t \right) -4\,At\sin \left( 4\,t \right) +B\sin\left( 4\,t \right) +4\,Bt\cos \left( 4\,t \right) \\
		y_p'' &= -8\,A\sin \left( 4\,t \right) -16\,At\cos \left( 4\,t \right) +8\,B\cos \left( 4\,t \right) -16\,Bt\sin \left( 4\,t \right) 
	\end{align*}
By plugging in the particular solution:
		$$
		y_p'' + 16yp = -8\,A\sin \left( 4\,t \right) +8\,B\cos \left( 4\,t \right) = -16\sin(4t)
		$$
		$$
		A = 2, B = 0
		$$
Thus the particular solution is: 
	$$
	y_p = 2t\cos \left( 4\,t \right)
	$$
\\
To find the eigenvalues, we can write the equation like below and solve for $\lambda$.
	\begin{align*}
		\lambda^2 + 16 &= 0
		\lambda^2 &= -16 \\
		\lambda &= \pm 4i
	\end{align*}
So we can now right this in its homogeneous solution form using $\lambda = 0 \pm 4i$
	\begin{align*}
		y_h = c_1\cos(4t) + c_2\sin(4t)
	\end{align*}
Thus the complete solution is 
	$$
	y(t) = c_1\cos(4t) + c_2\sin(4t) + 2t\cos \left( 4\,t \right)
	$$


\newpage

\noindent \textbf{Problem 15: }Write a complete solution with details on how you found the general solution
	$$
	y''- 10y' + 25y = -10.5e^{5t}
	$$
To solve for the particular solution, we can write $y_p$ as below
	\begin{align*}
		y_p &= A{t}^{2}{{e}^{5\,t}} \\
		y_p' &= 2\,At{{e}^{5\,t}}+5\,A{t}^{2}{{e}^{5\,t}} \\
		y_p'' &= 2\,A{{e}^{5\,t}}+20\,At{{e}^{5\,t}}+25\,A{t}^{2}{{e}^{5\,t}} \\
	\end{align*}
By plugging in the particular solution:
		$$
		y_p'' - 10y_p' + 25yp = 2\,A{{e}^{5\,t}} = -10.5e^{5t}
		$$
		$$
		A = \frac{-2}{10.5}
		$$
Thus the particular solution is: 
$$
y_p = \frac{-2}{10.5}{t}^{2}{{e}^{5\,t}}
$$
To find the eigenvalues, we can write the equation like below and solve for $\lambda$.
	\begin{align*}
		\lambda^2 - 10\lambda + 25 &= 0 \\
		(\lambda - 5)^2 &= 0 \\
		\lambda &= 5
	\end{align*}
So we can now right this in its homogeneous solution form using $\lambda = 5$
	\begin{align*}
	y_h = c_1e^{5t} + c_2te^{5t}
	\end{align*}
Thus the complete solution is 
	$$
	y(t) = c_1e^{5t} + c_2te^{5t} + \frac{-2}{10.5}{t}^{2}{{e}^{5\,t}}
	$$

\newpage 

\noindent \textbf{Problem 16: }Write a complete solution with details on how you found the general solution
	$$
	y'' - 7y' + 12y = -288t^3
	$$
To solve for the particular solution, we can write $y_p$ as below
	\begin{align*}
		y_p &= A{t}^{3}+B{t}^{2}+Ct+D \\
		y_p' &= 3\,A{t}^{2}+2\,Bt+C \\
		y_p'' &= 6\,At+2\,B
	\end{align*}
By plugging in the particular solution:
	\begin{align*}
	y_p'' -7y_p' + 12y_p &= (12A)t^3 + (-21A + 12B)t^2 + (6A -14B + 12C)t + (2B - 7C + 12D) \\
	&= -288t^3
	\end{align*}
	$$
	\text{rref}
	\begin{pmatrix}
		12 & 0 & 0 & 0 & -288 \\
		-21 & 12 & 0 & 0 & 0 \\
		6 & -14 & 12 & 0 & 0 \\
		0 & 2 & -7 & 12 & 0
	\end{pmatrix}
	= 
	\begin{pmatrix}
		1 & 0 & 0 & 0 & -24 \\
		0 & 1 & 0 & 0 & -42 \\
		0 & 0 & 1 & 0 & -37 \\
		0 & 0 & 0 & 1 & -14.5833
	\end{pmatrix}
	$$
Thus the particular solution is: 
	$$
	y_p = -24{t}^{3}+-42{t}^{2}+-37t+-14.5833
	$$
To find the eigenvalues, we can write the equation like below and solve for $\lambda$.
	\begin{align*}
		\lambda^2 - 7\lambda + 12 &= 0 \\
		(\lambda - 3)(\lambda  - 4) &= 0 \\
		\lambda &= 3, 4
	\end{align*}
So we can now right this in its homogeneous solution form using $\lambda = 3, 4$
	\begin{align*}
		y_h = c_1e^{3t} + c_2e^{4t}
	\end{align*}
Thus the complete solution is 
	$$
	y(t) = c_1e^{3t} + c_2e^{4t} + -24{t}^{3}+-42{t}^{2}+-37t+-14.5833
	$$

\newpage 

\noindent \textbf{Problem 21: }Write a complete solution with details on how you found the general solution
	\begin{align*}
	x^2y'' + 13xy' + 36y = x^6 && y(1) = -8, y'(1) = -2
	\end{align*}
Let the following be true:
	\begin{align*}
		y &= x^r &&&
		y' &= rx^{r-1} &&&
		y'' &= (r^2 - r)x^{r-2}
	\end{align*}
So then by plugging in the following into the homogeneous equation: 
	\begin{align*}
		x^2y'' + 13xy' + 36y &= x^r(r^2 - r + 13r + 36) = 0 \\
		&= x^r(r^2 + 12r + 36) = 0 \\
		&= x^r(r + 6)^2 = 0 \\
		& r = -6
	\end{align*}
So now we have the homogeneous solution: 
	$$
	y_h = (c_1 + c_2\ln|x|)x^{-6} 
	$$
To solve for the particular solution, we can write $y_p$ as below
	\begin{align*}
		y_p &= Ax^6 \\
		y_p' &= 6\,A{x}^{5} \\
		y_p'' &= 30\,A{x}^{4}
	\end{align*}
By plugging in the particular solution:
	$$
	x^2y_p'' + 13xy_p' + 36y_p = 144\,A{x}^{6} = x^6
	$$
	$$
	A = \frac{1}{144}
	$$
Thus the particular solution is: 
	$$
	y_p = \frac{1}{144}x^6
	$$
We can now have the complete solution, $y(t)$ to this differential equation:
	$$
	y(t) = (c_1 + c_2\ln|x|)x^{-6}  + \frac{1}{144}x^6
	$$
We now use $y'(t)$ and the initial conditions to solve for $c_1$ and $c_2$
	$$
	y'(t) = -6c_1x^{-7} + -6c_2\ln|x|x^{-7}  + c_2x^{-7} + \frac{6}{144}x^5
	$$
	\begin{align*}
		y(1) = c_1 + \frac{1}{144} = -8 && c_1 = -8 + -\frac{1}{144} = \frac{-1153}{144} \\
		y'(1) = -6c_1 + c_2 + \frac{6}{144} = -2 && c_2 = -2 + -\frac{6}{144} + \frac{6(-1153)}{144} = \frac{-601}{12}
	\end{align*}
Thus the solution is: 
	$$
	y(t) = \left(\frac{-1153}{144} + \frac{-601}{12}\ln|x|\right)x^{-6} + \frac{1}{144}x^6
	$$
	
\newpage 

\noindent \textbf{Problem 22: }Write a complete solution with details on how you found the general solution
	$$
	y'' - 4y' + 4y = \frac{16.5e^{2t}}{t^2 + 1}
	$$
To find the eigenvalues, we can write the equation like below and solve for $\lambda$.
	\begin{align*}
		\lambda^2  -4\lambda + 4 &= (\lambda - 2)^2 = 0 	\\
		\lambda &= 2 				
	\end{align*}
Now we can write the homogeneous solution as: 
	$$
	y_h = c_1e^{2t} + c_2te^{2t}
	$$
We can now generalize it to:
	$$
	y(t) = u_1(t)e^{2t} + u_2(t)te^{2t}
	$$
We now set the following to be true"
	$$
	u_1'(t)e^{2t} + u_2'(t)te^{2t} = 0
	$$
Now we take the first and second derivative of $y(t)$:
	\begin{align*}
		y'(t) &= u_1'(t)e^{2t} + 2u_1(t)e^{2t} + u_2'(t)te^{2t} + u_2(t)e^{2t} + 2u_2(t)te^{2t} \\
		&= 2u_1(t)e^{2t} + u_2(t)e^{2t} + 2u_2(t)te^{2t} \\
		y''(t) &= 2u_1'(t)e^{2t} +4u_1(t)e^{2t} + u_2'(t)e^{2t} + 4u_2(t)e^{2t} + 2u_2'(t)te^{2t} + 4u_2(t)te^{2t} \\
		&= 4u_1(t)e^{2t} + u_2'(t)e^{2t} + 4u_2(t)e^{2t} + 4u_2(t)te^{2t} \\
	\end{align*}
By plugging into the differential equation now:
	\begin{align*}
		y'' - 4y' + 4y &= 4u_1(t)e^{2t} + u_2'(t)e^{2t} + 4u_2(t)e^{2t} + 4u_2(t)te^{2t} \\
		&\text{ } -8u_1(t)e^{2t} + -4u_2(t)e^{2t} + -8u_2(t)te^{2t}\\
		&\text{ } + 4u_1(t)e^{2t} + 4u_2(t)te^{2t} \\
		&= u_2'(t)e^{2t}
	\end{align*}
	
\newpage

\noindent So now we solve for the $u_1(t)$ and $u_2(t)$
	\begin{align*}
		u_2'(t)e^{2t} &= \frac{16.5e^{2t}}{t^2 + 1} \\
		u_2'(t) &= \frac{16.5}{t^2 + 1} \\
		u_2(t) &= 16.5\arctan(t) + c_2
	\end{align*}
	\begin{align*}
		u_1'(t)e^{2t} + u_2'(t)te^{2t} &= 0 \\
		u_1'(t)e^{2t} &= -u_2'(t)te^{2t} \\
		&= \frac{-16.5te^{2t}}{t^2 + 1} \\
		u_1'(t) &= \frac{-16.5t}{t^2 + 1} \\
		u_1(t) &= \frac{-16.5}{2}\ln(t^2 + 1) + c_1
	\end{align*}
Now we take our generalized solution and plug everything in:
	\begin{align*}
		y(t) &= \frac{-16.5}{2}\ln(t^2 + 1)e^{2t} + c_1e^{2t} + 16.5\arctan(t)te^{2t} + c_2te^{2t} \\
		&= c_1e^{2t} + c_2te^{2t} + \frac{-16.5}{2}\ln(t^2 + 1)e^{2t} + 16.5\arctan(t)te^{2t}
	\end{align*}
	
	
	
	
	
	
	
	
	
	
	
\end{document}
